[new] updates on program algebra.

testGCD.v
@@ -1,11 +1,13 @@
-From PA Require Import ProgramAlgebra.
+From PA Require Import ProgramAlgebraAlt.
+Import ProgramAlgebraAlt.
 Import Nat.
 Import List.
 Require Import String.
 Import ListNotations.
 
+Open Scope alg_scope.
 
-Variable bot : Type.
+Print Visibility.
 
 Record MyVar := mkVar {
   id: string;
@@ -15,78 +17,162 @@ Record MyVar := mkVar {
 Definition eqVarb (x y : MyVar) := 
   andb (eqb x.(id) y.(id)) (PeanoNat.Nat.eqb x.(val) y.(val)).
 
-Definition GLOBVARS := [(mkVar "a" 10);(mkVar "b" 4)].
+Variable GLOBVARS : list MyVar.
+
+Definition Constraint : Prop := forall a b, GLOBVARS = [a;b].
 
 Definition UNDEF := mkVar "Undefined" 0.
 
-Instance myParams : ProgramAlgebra.UserParams :=
-  ProgramAlgebra.Build_UserParams MyVar GLOBVARS eqVarb.
+Instance myParams : UserParams :=
+  Build_UserParams MyVar GLOBVARS eqVarb Constraint.
 
-Axiom equalGLOB : GLOBVARS = ProgramAlgebra.GLOBVARS.
+Search "eqb".
 
-Axiom equalB : eqVarb = ProgramAlgebra.eqb.
-
-Notation "|-| l" := (ProgramAlgebra.Choice_of_Alg_List l)(at level 20).
-
-Notation "_|_" := (ProgramAlgebra.Chaos)(at level 10).
-
-Notation "@{ e }" := (fun x => ProgramAlgebra.Assn x e)(at level 10).
-
-Definition eqz_b : ProgramAlgebra.Boolexp :=
-  fun l =>
-    match (find (fun x => eqb x.(id) "b") l) with
-    | Some x => if (PeanoNat.Nat.eqb x.(val) 0) then false else true
-    | _ => false
-    end.
-
-Definition gcd_step := ProgramAlgebra.makeAssign ProgramAlgebra.GLOBVARS
-  (fun l =>
-   match (find (fun x => eqb x.(id) "a") l),
-    (find (fun x => eqb x.(id) "b") l) with
-   | Some x, Some y => [(mkVar x.(id) y.(val));(mkVar y.(id) (modulo x.(val) y.(val)))]
-   | _, _ => []
-   end).
-
-Definition skip := ProgramAlgebra.makeAssign ProgramAlgebra.GLOBVARS
-  (fun l => l).
-
-Fixpoint mapid {s} (x : ProgramAlgebra.Alg s) :=
-  match x with
-  | ProgramAlgebra.Assn _ a => @{a} (ProgramAlgebra.Alg s)
-  | ProgramAlgebra.Choice _ P Q =>
-     ProgramAlgebra.Choice (ProgramAlgebra.Alg s) (mapid P) (mapid Q)
-  | ProgramAlgebra.Chaos _ => _|_ (ProgramAlgebra.Alg s)
-  | ProgramAlgebra.Seq _ P Q =>
-     ProgramAlgebra.Choice (ProgramAlgebra.Alg s) (mapid P) (mapid Q)
-  | ProgramAlgebra.Cond _ P b Q =>
-     ProgramAlgebra.Cond (ProgramAlgebra.Alg s) (mapid P) b (mapid Q)
-  | ProgramAlgebra.Recur _ f => _|_ (ProgramAlgebra.Alg s)
+Definition hdeqz : Boolexp :=
+ fun l =>
+  match (hd_error l) with
+  | None => false
+  | Some x => x.(val) =? 0
   end.
 
-Definition testIter {s} (x : ProgramAlgebra.Alg s) :=
-  ProgramAlgebra.Seq (ProgramAlgebra.Alg s)
-  (mapid x) (ProgramAlgebra.Cond (ProgramAlgebra.Alg s)
-     (@{gcd_step} (ProgramAlgebra.Alg s)) eqz_b
-     (@{skip} (ProgramAlgebra.Alg s))).
+Definition skip := @{ empty_assn }.
 
-Definition testRec := ProgramAlgebra.Recur (ProgramAlgebra.Alg bot) testIter.
+Definition GCDFunc (l : list Var)  : list Var := 
+  let a := hd UNDEF l in let b := hd UNDEF (tl l) in
+  [(mkVar a.(id) (b.(val) mod a.(val)));(mkVar b.(id) a.(val))].
 
-Definition testnf := @{ ProgramAlgebra.makeAssign ProgramAlgebra.GLOBVARS 
-  (fun l => [(mkVar "a" 2);(mkVar "b" 0)]) } bot.
+Definition GCDAssn := @{ makeAssign GLOBVARS GCDFunc}.
 
-Variable lub : ProgramAlgebra.Closure -> ProgramAlgebra.Ualg.
+Definition GCDStep (a : Alg) : Alg :=
+  (skip <| hdeqz |> (GCDAssn ;; a)).
+(**TODO*)
 
-Example testlim : testIter testnf = testRec .
-Proof. unfold testRec. rewrite ProgramAlgebra.Recur_clos with (lub := lub).
-rewrite ProgramAlgebra.fix_is_lub with (lub := lub);auto.
-unfold ProgramAlgebra.RecurFix. unfold testnf. eexists. split.
-unfold testIter. unfold skip. unfold gcd_step.
-rewrite ProgramAlgebra.Assign_Cond. unfold mapid.
-rewrite ProgramAlgebra.Assign_compose. reflexivity.
-unfold eqz_b. unfold ProgramAlgebra.exp_Cond.
-simpl. unfold ProgramAlgebra.eqEval. auto.
+Definition GCDStr := Recur GCDStep (_|_).
+
+Ltac CH_check := unfold CH;intros;try contradiction.
+
+Ltac pauto := auto with palg.
+
+Definition GCDRes := let a := hd UNDEF GLOBVARS in
+  let b := hd UNDEF (tl GLOBVARS) in
+  @{ GLOBVARS :== fun x => [(mkVar a.(id) 0);(mkVar b.(id) (PeanoNat.Nat.gcd a.(val) b.(val)))]}.
+
+Lemma GcdBase : FNFPres (_|_) (GCDStep (_|_)).
+Proof.
+  unfold FNFPres. do 2 eexists. assert (skip = |-|[skip]) by auto.
+  split;try split. apply (Chaos_to_NF []).
+  unfold FNF. do 2 eexists. split;auto. CH_check.
+  unfold GCDStep. split. pose (Chaos_zero_Seq_r GCDAssn).
+  pose (rwt_comb _ _ _ _ (CDC hdeqz) (rwt_refl skip) r ).
+  apply (rwt_trans _ _ _ r0). apply Cond_rev. unfold FNF.
+  do 2 eexists. rewrite H. split;auto. CH_check.
+  destruct H0; try contradiction. rewrite <- H0. unfold skip.
+  eexists;split;pauto. unfold Refine. do 4 eexists. split; try split.
+  3:split. 3: rewrite H. 1,3:reflexivity. 1,2 : CH_check.
+  destruct H0;try contradiction. rewrite <- H0.
+  unfold skip. eexists;split;pauto. intros. right. auto.
 Qed.
 
+Hypothesis GcdStable : forall x, FNFPres (GCDStep x) (GCDStep (GCDStep x)).
 
+(*  intros. unfold GCDStep. unfold FNFPres. assert (skip = |-|[skip]) by auto.
+  assert (CH [@{ GLOBVARS :== GCDFunc}]). CH_check. destruct H0;try contradiction.
+  rewrite <- H0. eexists;split;pauto. assert (CH [skip]). CH_check. unfold skip in *.
+  destruct H1;try contradiction. rewrite <- H1. eexists;split;pauto. 
+  destruct x.
+  - destruct a.
+    + pose (Chaos_zero_Seq_r GCDAssn).
+      pose (rwt_comb _ _ _ _ (CDC hdeqz) (rwt_refl skip) r).
+      pose (Cond_rev skip (_|_) hdeqz).
+      pose (rwt_trans _ _ _ r0 r1). 
+      do 2 eexists. split; split. 3 : split. apply r2.
+      unfold FNF. rewrite H. do 2 eexists; split; pauto.
+      unfold GCDAssn in r2. unfold GCDAssn.
+      pose (Assign_to_NF GLOBVARS GCDFunc). rewrite H in r2.
+      rewrite H. pose (rwt_comb _ _ _ _ Seq r3 r2).
+      pose (NF_over_Seq [@{ GLOBVARS :== GCDFunc}] [skip] false_stat 
+        (fun g => negb (hdeqz g))). apply r5 in H0 as H2;auto.
+      pose (rwt_trans _ _ _ r4 H2). clear r5.
+      pose (Seq_over_Choice [@{ GLOBVARS :== GCDFunc}] [skip]).
+      apply r5 in H1 as H3;auto. clear r5.
+      pose (rwt_comb _ _ _ _ (CDC (fun g : list Var =>
+        (false_stat g || CH_over_Boolexp [@{ GLOBVARS :== GCDFunc}]
+        (fun g0 : list Var => negb (hdeqz g0)))%bool)) (rwt_refl (_|_)) H3).
+      pose (rwt_trans _ _ _ r6 r5).
+      assert (|-| [skip] <--> (_|_) <| false_stat |> |-| [skip]).
+      rewrite <- H. unfold skip. unfold empty_assn. 
+      pose (Assign_to_NF GLOBVARS refl_exp). apply (rwt_trans _ _ _ r8).
+      apply rwt_comb;pauto. pose (rwt_comb _ _ _ _ (CDC hdeqz) H4 r7).
+      apply (rwt_trans _ _ _ r8). clear r8 r7 r6 r5 r4 r3 r2 r1 r0 r.
+      clear H4 H3 H2. simpl. pose (NF_over_Cond [skip] [@{ GLOBVARS :== GCDFunc};; skip].
+      CH_check. destruct H0;try contradiction. rewrite <- H0.
+      unfold skip. eexists;split;pauto. 
+*)
 
+(*Proof.
+  intros. unfold FNFPres. pose (FNF_closure x).
+  pose (FNF_closure (GCDStep x)). destruct e. destruct e0.
+  exists x0. exists x1. split;auto.
+Qed.*)
+
+Lemma GcdStrPres : AlgPres GCDStr.
+Proof. apply AlgPresInd. apply GcdBase. apply GcdStable. Qed.
+
+Lemma GcdReachRes : SthExists GCDRes GCDStr.
+Abort.
+(*
+Proof.
+  unfold Lub. split.
+  - apply AlgPresInv;auto. apply GcdPres.
+  - unfold FixExists. apply Streams.Further. apply Streams.Here.
+    unfold GCDStep. simpl. unfold FixStep. unfold GCDRes.
+    split;simpl. all : apply rwt_comm; unfold GCDAssn.
+    + pose (Assign_Seq GLOBVARS GCDFunc refl_exp).
+      pose (rwt_comb (@{ GLOBVARS :== refl_exp}) _ _ _ (CDC hdeqz)
+       (rwt_refl (@{ GLOBVARS :== refl_exp})) r).
+      apply (rwt_trans _ _ _ r0). clear r r0.
+      pose (Assign_Cond GLOBVARS refl_exp (fun x : list Var =>
+       refl_exp (GCDFunc x)) hdeqz). apply (rwt_trans _ _ _ r).
+      clear r. apply eval_equiv. unfold eqEval. simpl. auto.
+    + pose (Assign_Seq GLOBVARS GCDFunc refl_exp).
+      pose (rwt_comb (@{ GLOBVARS :== refl_exp}) _ _ _ (CDC hdeqz)
+       (rwt_refl (@{ GLOBVARS :== refl_exp})) r).
+      pose (Assign_Cond GLOBVARS refl_exp (fun x : list Var =>
+       refl_exp (GCDFunc x)) hdeqz).
+      pose (rwt_trans _ _ _ r0 r1).
+      pose (rwt_comb _ _ _ _ Seq (rwt_refl (@{ GLOBVARS :== GCDFunc}))
+       r2). pose (Assign_Seq GLOBVARS GCDFunc (exp_Cond refl_exp (fun x 
+       => refl_exp (GCDFunc x)) hdeqz)). pose (rwt_trans _ _ _ r3 r4).
+      pose (rwt_comb _ _ _ _ (CDC hdeqz) r2 r5).
+      apply (rwt_trans _ _ _ r6). clear r r0 r1 r2 r3 r4 r5 r6.
+      pose (Assign_Cond GLOBVARS (exp_Cond refl_exp (fun x=> refl_exp (GCDFunc x)) hdeqz)
+        (fun x => exp_Cond refl_exp (fun x0 : list Var => refl_exp (GCDFunc x0))
+         hdeqz (GCDFunc x)) hdeqz). apply (rwt_trans _ _ _ r).
+      clear r. apply eval_equiv. unfold eqEval. simpl. auto.
+Qed.*)
+
+Definition falg := (_|_).
+
+Lemma refinegcd : exists r s, (r <--> falg /\ FNF r) /\ 
+   (s <--> GCDRes /\ FNF s) /\ Refine r s.
+Abort.
+Proof.
+  do 2 eexists. split;try split;try split.
+  - apply rwt_comm. unfold GCDRes. apply (Assign_to_NF _ _ false_stat).
+    auto.
+  - unfold FNF. do 2 eexists. split;eauto. unfold CH. intros.
+    destruct H; try contradiction. rewrite <- H. eexists;split;try apply rwt_refl.
+    unfold Total_Assign. auto. 
+  - apply rwt_comm. unfold altGcd. apply (Assign_to_NF _ _ false_stat).
+    auto.
+  - unfold FNF. do 2 eexists. split;eauto. unfold CH. intros.
+    destruct H;try contradiction. rewrite <- H. eexists;split;try apply rwt_refl.
+    unfold Total_Assign. auto. 
+  - unfold Refine. do 4 eexists; eauto. split;try split;try split;try reflexivity.
+    1,2 : unfold CH;intros;destruct H;try contradiction; rewrite <- H; eexists;split;
+    try apply rwt_refl;unfold Total_Assign; auto. left. split;auto.
+    unfold RefineCH. intros. destruct H; try contradiction. rewrite <- H.
+    eexists. split. unfold In. left. reflexivity. unfold eqAssn. unfold eqEval.
+    simpl.  auto.
+Qed.
 
