testAlt.v
@@ -1,0 +1,164 @@
+From PA Require Import ProgramAlgebraAlt.
+Import ProgramAlgebraAlt.
+Require Import Lia.
+Import Nat.
+Import List.
+Require Import String.
+Import ListNotations.
+
+Open Scope alg_scope.
+
+Print Visibility.
+
+Record MyVar := mkVar {
+  id: string;
+  val : nat;
+}.
+
+Definition eqbVar (x y : MyVar) := 
+  andb (eqb x.(id) y.(id)) (PeanoNat.Nat.eqb x.(val) y.(val)).
+
+Variable GLOBVARS : list MyVar.
+
+Definition Constraint := exists a b c, (PeanoNat.Nat.leb a.(val) 10 = true)
+ /\ (eqbVar a b = false) /\ (eqbVar a c = false) /\ (eqbVar b c = false) /\ GLOBVARS = [a;b;c].
+
+Lemma eqbVar_sym : forall x y, eqbVar x y = eqbVar y x.
+Proof. intros. unfold eqbVar. destruct x. destruct y. simpl.
+  assert ((id0 =? id1) % string = (id1 =? id0) %string) by apply eqb_sym.
+  assert ((val0 =? val1) = (val1 =? val0)) by apply PeanoNat.Nat.eqb_sym.
+  rewrite H. rewrite H0. auto. Qed.
+
+Definition UNDEF := mkVar "Undefined" 0.
+
+Instance myParams : UserParams :=
+  Build_UserParams MyVar GLOBVARS eqbVar Constraint.
+
+Fixpoint ascending (l : list Var) : list Var :=
+  match l with
+  | [] => []
+  | h :: tl => (mkVar h.(id) (h.(val) + 1)) :: ascending tl
+  end.
+
+Fixpoint descending (l : list Var) : list Var :=
+  match l with
+  | [] => []
+  | h :: tl => (mkVar h.(id) (h.(val) - 1)) :: descending tl
+  end.
+
+Definition dscassn := makeAssign GLOBVARS descending.
+
+Definition ascassn := makeAssign GLOBVARS ascending.
+
+Definition hdge2 : Boolexp :=
+ fun l =>
+  match (hd_error l) with
+  | None => false
+  | Some x => if (PeanoNat.Nat.leb 20 x.(val)) then true else false
+  end.
+
+Definition testAlg := (@{ascassn}) ;;
+  ((@{ascassn}) <| hdge2  |> (@{dscassn})).
+
+Definition testAlg2 := (_|_) <| hdge2 |>
+  (@{ascassn}) ;; ((|-|[@{ascassn};@{dscassn}])).
+
+Definition testassn := Lift (Assn
+  {|
+    ids := GLOBVARS;
+    values :=
+      fun x =>
+       exp_Cond ascending descending hdge2
+       (ascending x)
+  |}).
+
+Definition testnf :=
+ (_|_) <| false_stat |> (|-| [testassn]).
+
+Ltac rwt_step := apply rwt_comb;auto;try apply rwt_refl.
+
+Lemma nf : testAlg <--> testnf.
+Proof.
+  unfold testAlg. unfold testnf. unfold ascassn. unfold dscassn.
+  apply (rwt_trans _ (@{ ProgramAlgebraAlt.GLOBVARS :== ascending } ;;
+     (@{ ProgramAlgebraAlt.GLOBVARS :== exp_Cond ascending descending hdge2 }))).
+  rwt_step. apply Assign_Cond.
+  pose (Assign_Seq GLOBVARS ascending (exp_Cond ascending descending hdge2)).
+  simpl in r. apply (rwt_trans _ _ _ r). clear r.
+  pose (Assign_to_NF GLOBVARS (fun x => exp_Cond ascending descending hdge2
+       (ascending x))). simpl in r.
+  assert(|-|[testassn] = testassn) by auto. rewrite H.
+  unfold testassn. apply r.
+Qed.
+
+Definition testassn2_1 := Lift (Assn
+  {|
+    ids := GLOBVARS;
+    values :=
+      fun x  => ascending (ascending x)
+  |}).
+
+Definition testassn2_2 := Lift (Assn
+   {|
+     ids := GLOBVARS;
+     values := fun x => descending (ascending x)
+   |}).
+
+Definition testnf2 :=
+  (_|_) <| hdge2 |> (|-|[testassn2_1;testassn2_2]).
+
+Lemma nf2 : testAlg2 <--> testnf2.
+Proof.
+  unfold testAlg2. unfold testnf2. unfold ascassn. unfold dscassn.
+  rwt_step. assert (GLOBVARS = ProgramAlgebraAlt.GLOBVARS) by auto.
+  repeat rewrite H. remember (|-| [@{ ProgramAlgebraAlt.GLOBVARS :== ascending};
+     @{ ProgramAlgebraAlt.GLOBVARS :== descending}]). rewrite <- H.
+  assert (@{ GLOBVARS :== ascending} = |-| [@{ GLOBVARS :== ascending}]) by auto.
+  rewrite H0. rewrite Heqa. repeat rewrite <- H. clear Heqa. clear H0.
+  pose (Seq_over_Choice [@{ GLOBVARS :== ascending}]
+   [@{ GLOBVARS :== ascending};@{ GLOBVARS :== descending}]).
+  apply (rwt_trans _ (|-|(map (fun g : Alg * Alg => fst g;; snd g) (list_prod
+    [@{ ProgramAlgebraAlt.GLOBVARS :== ascending}]
+    [@{ ProgramAlgebraAlt.GLOBVARS :== ascending};
+    @{ ProgramAlgebraAlt.GLOBVARS :== descending}])))).
+  apply r. 1,2 : unfold CH;intros; destruct H0. 2: destruct H0.
+  all : try contradiction. all : try (eexists; rewrite H0; split; try apply rwt_refl;
+  pauto). destruct H0; try contradiction. rewrite  <- H0.
+  eexists;split;pauto. clear r. unfold list_prod. simpl. unfold testassn2_1.
+  unfold testassn2_2. rwt_step;apply Assign_Seq.
+Qed.
+
+Example testrefine : Refine testnf2 testnf.
+Proof. 
+  unfold Refine. unfold testnf. unfold testnf2.
+  do 4 eexists. split;split;try split. 
+  - unfold CH. intros. destruct H.
+    + unfold testassn2_1 in H. eexists. split. rewrite <- H. apply rwt_refl.
+      unfold Total_Assign. auto.
+    + destruct H;try contradiction. unfold testassn2_2 in H. eexists. split.
+      rewrite <- H. all : pauto.
+  - reflexivity.
+  - unfold CH. intros. destruct H;try contradiction. unfold testassn in H.
+    eexists. split;try rewrite <- H;pauto.
+  - simpl in *. unfold Constraint. intros. do 4 destruct H. destruct H0.
+    destruct H1. destruct H2. unfold false_stat. left. split;auto.
+    unfold RefineCH. intros. destruct H4; try contradiction. rewrite <- H4.
+    unfold testassn. exists testassn2_2. split.
+    + unfold In. right. left. reflexivity.
+    + assert (forall x, eqbVar x x = true). { intros. unfold eqbVar. destruct x3.
+      simpl. apply Bool.andb_true_iff. split. apply eqb_refl. apply PeanoNat.Nat.eqb_refl. }
+      unfold testassn2_1. unfold eqAssn. unfold eqEval. rewrite H3. simpl.
+      unfold extends_mapping. unfold extends_mapping_help. simpl. rewrite H3.
+      simpl. repeat rewrite H5. pose (eqbVar_sym x0 x). pose (eqbVar_sym x1 x).
+      pose (eqbVar_sym x1 x0). rewrite H0 in e. rewrite H1 in e0. rewrite H2 in e1.
+      rewrite e. rewrite e0. rewrite e1. unfold exp_Cond. unfold hdge2.
+      pose (PeanoNat.Nat.leb_spec0 (val x) 10). apply Bool.reflect_iff in r.
+      apply r in H. assert ((val x) + 1 < 20). lia. pose (PeanoNat.Nat.ltb_spec0 (val x + 1) 20).
+      apply Bool.reflect_iff in r0. rewrite r0 in H6.
+      rewrite PeanoNat.Nat.ltb_antisym in H6. rewrite Bool.negb_true_iff in H6.
+      unfold hd_error. assert (val x + 1 = val {| id := id x; val := val x + 1 |}) by auto.
+      rewrite <- H7. rewrite H6. simpl. auto. 
+Qed.
+
+
+
