testAlt2.v
@@ -1,0 +1,148 @@
+From PA Require Import ProgramAlgebraAlt.
+Import ProgramAlgebraAlt.
+Import Nat List.
+Require Import String.
+Import ListNotations.
+
+Open Scope alg_scope.
+
+Print Visibility.
+
+Record Position := mkPos {
+  hor : nat;
+  ver : nat;
+}.
+
+Record MyVar := mkVar {
+  id: string;
+  val : Position;
+}.
+
+Definition eqbPos (x y : Position) :=
+  andb (PeanoNat.Nat.eqb x.(hor) y.(hor))
+       (PeanoNat.Nat.eqb x.(ver) y.(ver)).
+
+Definition eqbVar (x y : MyVar) := 
+  andb (eqb x.(id) y.(id)) (eqbPos x.(val) y.(val)).
+
+Definition GLOBVARS := [(mkVar "start" {|hor:=0;ver:=0|});
+  (mkVar "mid" {|hor:=5;ver:=5|});(mkVar "end" {|hor:=10;ver:=10|})].
+
+Definition UNDEF := mkVar "Undefined" {|hor:=0;ver:=0|}.
+
+Instance myParams : UserParams :=
+  Build_UserParams MyVar GLOBVARS eqbVar.
+
+Fixpoint shift (l : list Var) : list Var :=
+  match l with
+  | [] => []
+  | h :: tl => (mkVar h.(id) (mkPos (h.(val).(hor)+1) h.(val).(ver))) :: shift tl
+  end.
+
+Definition reverse (l : list Var) : list Var :=
+  let h := hd UNDEF l in let k := nth 1 l UNDEF in
+  let t := nth 2 l UNDEF in
+  (mkVar h.(id) t.(val)) :: (k :: [mkVar t.(id) h.(val)]).
+
+Fixpoint unshift (l : list Var) : list Var :=
+  match l with
+  | [] => []
+  | h :: tl => (mkVar h.(id) (mkPos (h.(val).(hor)-1) h.(val).(ver))) :: unshift tl
+  end.
+
+Definition shassn := makeAssign GLOBVARS shift.
+
+Definition revassn := makeAssign GLOBVARS reverse.
+
+Definition unshassn := makeAssign GLOBVARS unshift.
+
+
+
+Definition testAlg := (@{ascassn}) ;;
+  ((@{ascassn}) <| hdge2  |> (@{dscassn})).
+
+Definition testAlg2 := (_|_) <| hdge2 |>
+  ((|-|[@{ascassn};@{dscassn}]) ;; (@{ascassn})).
+
+Definition testassn := Lift (Assn
+  {|
+    ids := GLOBVARS;
+    values :=
+      fun x =>
+       exp_Cond ascending descending hdge2
+       (ascending x)
+  |}).
+
+Definition testnf :=
+ (_|_) <| false_stat |> (|-| [testassn]).
+
+Ltac rwt_step := apply rwt_comb;auto;try apply rwt_refl.
+
+Lemma nf : testAlg <--> testnf.
+Proof.
+  unfold testAlg. unfold testnf. unfold ascassn. unfold dscassn.
+  apply (rwt_trans _ (@{ ProgramAlgebraAlt.GLOBVARS :== ascending } ;;
+     (@{ ProgramAlgebraAlt.GLOBVARS :== exp_Cond ascending descending hdge2 }))).
+  rwt_step. apply Assign_Cond.
+  pose (Assign_Seq GLOBVARS ascending (exp_Cond ascending descending hdge2)).
+  simpl in r. apply (rwt_trans _ _ _ r). clear r.
+  pose (Assign_to_NF GLOBVARS (fun x => exp_Cond ascending descending hdge2
+       (ascending x)) false_stat). simpl in r.
+  assert(|-|[testassn] = testassn) by auto. rewrite H.
+  unfold testassn. apply r. auto.
+Qed.
+
+Definition testassn2_1 := Lift (Assn
+  {|
+    ids := GLOBVARS;
+    values :=
+      fun x  => ascending (ascending x)
+  |}).
+
+Definition testassn2_2 := Lift (Assn
+   {|
+     ids := GLOBVARS;
+     values := fun x => ascending (descending x)
+   |}).
+
+Definition testnf2 :=
+  (_|_) <| hdge2 |> (|-|[testassn2_1;testassn2_2]).
+
+Lemma nf2 : testAlg2 <--> testnf2.
+Proof.
+  unfold testAlg2. unfold testnf2. unfold ascassn. unfold dscassn.
+  rwt_step. assert (GLOBVARS = ProgramAlgebraAlt.GLOBVARS) by auto.
+  repeat rewrite H. remember (|-| [@{ ProgramAlgebraAlt.GLOBVARS :== ascending};
+     @{ ProgramAlgebraAlt.GLOBVARS :== descending}]). rewrite <- H.
+  assert (@{ GLOBVARS :== ascending} = |-| [@{ GLOBVARS :== ascending}]) by auto.
+  rewrite H0. rewrite Heqa. repeat rewrite <- H. clear Heqa. clear H0.
+  pose (Seq_over_Choice [@{ GLOBVARS :== ascending};@{ GLOBVARS :== descending}]
+    [@{ GLOBVARS :== ascending}]).
+  apply (rwt_trans _ (|-|(map (fun g : Alg * Alg => fst g;; snd g) (list_prod
+    [@{ ProgramAlgebraAlt.GLOBVARS :== ascending};
+    @{ ProgramAlgebraAlt.GLOBVARS :== descending}]
+    [@{ ProgramAlgebraAlt.GLOBVARS :== ascending}])))).
+  apply r. 1,2 : unfold CH;intros; destruct H0. 2: destruct H0.
+  all : try contradiction. all : try (eexists; rewrite H0; split; try apply rwt_refl;
+  unfold Total_Assign;auto). clear r. unfold list_prod. simpl. unfold testassn2_1.
+  unfold testassn2_2. rwt_step;apply Assign_Seq.
+Qed.
+
+Example testrefine : Refine testnf2 testnf.
+Proof. 
+  unfold Refine. unfold testnf. unfold testnf2.
+  do 4 eexists. split;split;try split. 
+  - unfold CH. intros. destruct H.
+    + unfold testassn2_1 in H. eexists. split. rewrite <- H. apply rwt_refl.
+      unfold Total_Assign. auto.
+    + destruct H;try contradiction. unfold testassn2_2 in H. eexists. split.
+      rewrite <- H. apply rwt_refl. unfold Total_Assign. auto.
+  - reflexivity.
+  - unfold CH. intros. destruct H;try contradiction. unfold testassn in H.
+    eexists. split. rewrite <- H. apply rwt_refl. unfold Total_Assign. auto.
+  - unfold false_stat. unfold GLOBVARS. simpl. left. split;auto.
+    unfold RefineCH. intros. destruct H; try contradiction. rewrite <- H.
+    unfold testassn. exists testassn2_1. split.
+    + unfold In. left. reflexivity.
+    + unfold testassn2_1. unfold eqAssn. unfold eqEval. simpl. intros. auto.
+Qed.
